(cramers-rule-section)=

:::{index} Cramer's rule
:::

# Cramer's rule

:::{figure} https://upload.wikimedia.org/wikipedia/commons/thumb/6/6d/Gabriel_Cramer.jpg/220px-Gabriel_Cramer.jpg
:width: 200
:alt: Gabriel Cramer
:figclass: margin

<a href="https://en.wikipedia.org/wiki/Gabriel_Cramer" target="_blank">Gabriel Cramer (1704 - 1752)</a>
:::
     
**Cramer's rule**, named after Swiss mathematician <a href="https://en.wikipedia.org/wiki/Gabriel_Cramer" target="_blank">Gabriel Cramer</a>, is an explicit rule for calculating the solution to a system of linear equations using determinants. We saw in the section on [determinants](determinant-section) that the solution to the system of linear equations

$$ \begin{pmatrix} a & b \\ c & d \end{pmatrix}
    \begin{pmatrix} x_1 \\ x_2 \end{pmatrix} =
    \begin{pmatrix} e \\ f \end{pmatrix}$$

is

$$ \begin{align*}
    x_1 &= \frac{de - bf}{ad - bc}, & \qquad
    x_2 &= \frac{af - ce}{ad - bc}.
\end{align*} $$

We can recognise that the solution to both variables includes the determinant of the coefficient matrix, $ad - bc$, in the denomimator. But what about the numerator? If we consider the solution to $x_1$ then in $de - bf$ we can see that the constant values $e$ and $f$ are included and we have the subtraction of two products which is similar to the determinant of a $2 \times 2$ matrix, i.e.,

$$ \begin{align*}
    de - bf = \begin{vmatrix} e & b \\ f & d \end{vmatrix}.
\end{align*} $$

Doing similar for the solution to $x_2$ we see that the numerator is

$$ \begin{align*}
    af - ce = \begin{vmatrix} a & e \\ c & f \end{vmatrix}.
\end{align*} $$

These determinants are simply the coefficient matrix $\begin{pmatrix} a & b \\ c & d \end{pmatrix}$ with first and second columns replaced by the constant vector $\begin{pmatrix} e \\ f \end{pmatrix}$ for $x_1$ and $x_2$ respectively. This can be extended to larger systems to give us Cramer's rule.

::::{prf:theorem} Cramer's rule
:label: cramers-rule-theorem

The solution to a non-singular linear system of equations of the form $A\mathbf{x}=\mathbf{b}$ can be calculated using Cramer's rule which is

$$ x_i = \frac{\det(A_i)}{\det(A)}, $$(cramers-rule-equation)

where $A_i$ is a matrix obtained by replacing column $i$ of $A$ with $\mathbf{b}$.
::::

:::{prf:proof}

(from <a href="https://proofwiki.org/wiki/Cramer%27s_Rule" target="_blank">Proof Wiki</a>)

The solution to a system of linear equations $A \mathbf{x} = \mathbf{b}$ can be calculated using $\mathbf{x} = A^{-1} \mathbf{b}$ where $A^{-1}$ is the inverse of the coefficient matrix $A$. The {prf:ref}`adjoint-determinant formula<adjoint-determinant-formula-theorem>` for calculating the inverse is

$$ A^{-1} = \frac{\operatorname{adj}(A)}{\det(A)}, $$

so

$$ \mathbf{x} = \frac{1}{\det(A)} \operatorname{adj}(A) \mathbf{b}. $$

Since $\operatorname{adj}(A) = C^T$ where $C$ is the matrix of {prf:ref}`co-factors<cofactor-definition>`

$$ C^T = \begin{pmatrix} 
    C_{11} & C_{21} & \cdots & C_{n1} \\
    C_{12} & C_{22} & \cdots & C_{n2} \\
    \vdots & \vdots & \ddots & \vdots \\
    C_{1n} & C_{2n} & \cdots & C_{nn}
\end{pmatrix}. $$

then for the $i$th element of $\mathbf{x}$ using the {prf:ref}`definition of matrix multiplication<matrix-multiplication-definition>` we have

$$ x_i = \frac{1}{\det(A)} \sum_{j=1}^n C_{ji} b_j $$

In Cramer's rule, $A_i$ is the matrix formed by replacing the $i$th column of $A$ with $\mathbf{b}$

$$ A_i = \begin{pmatrix}
        a_{11} & \cdots & a_{1,i-1} & b_1 & a_{1,i+1} & \cdots & a_{1n} \\
        a_{21} & \cdots & a_{2,i-1} & b_2 & a_{2,i+1} & \cdots & a_{2n} \\
        \vdots & \ddots & \vdots & \vdots & \vdots & \ddots & \vdots \\
        a_{n1} & \cdots & a_{n,i-1} & b_n & a_{n,i+1} & \cdots & a_{nn}
    \end{pmatrix}. $$

Since removing the $i$th column from both $A$ and $A_i$ (the one with the $b$ values) results in the same matrix then the cofactors of $A_i$ are the same as the cofactors of $A$. If we calculate $\det(A_i)$ by expanding along the $i$th column of $A_i$ then

$$ \det(A_i) = b_1 C_{1i} + b_2 C_{2i} + \cdots + b_n C_{ni} = \sum_{j=1}^n C_{ji} b_j, $$

so $x_i = \dfrac{\det(A_i)}{\det(A)}$.
:::

::::{prf:example}
:label: cramers-rule-example

Solve the following systems of linear equations using Cramer's rule

&emsp; (i) &emsp; $\begin{array}{rl}
    3x_1 - 2x_2 &= -4, \\
    x_1 - 3x_2 &= 1.
\end{array}$

:::{dropdown} Solution
Here $A = \begin{pmatrix} 3 & -2 \\ 1 & -3 \end{pmatrix}$ and $\mathbf{b} = \begin{pmatrix} -4 \\ 1 \end{pmatrix}$

$$ \begin{align*}
    x_1 &= \frac{
    \begin{vmatrix} -4 & -2 \\ 1 & -3 \end{vmatrix}}
    {\begin{vmatrix} 3 & -2 \\ 1 & -3 \end{vmatrix}} = \frac{14}{-7} = -2,  \\
    \\
    x_2 &= \frac{\begin{vmatrix} 3 & -4 \\ 1 & 1 \end{vmatrix}}{-7} = 
    \frac{7}{-7} = -1.
\end{align*} $$

Checking the solution

$$ \begin{align*}
    A\mathbf{x} = \begin{pmatrix} 3 & -2 \\ 1 & -3 \end{pmatrix}
    \begin{pmatrix} -2 \\ -1 \end{pmatrix} =
    \begin{pmatrix} -4 \\ 1 \end{pmatrix} = \mathbf{b} \qquad \checkmark
\end{align*} $$
:::

&emsp; (ii) &emsp; $\begin{array}{rl}
    -2x_1 - 3x_2 - x_3 &= -5, \\
    -4x_1 + 4x_2 + 3x_3 &= -20, \\
    -3x_1 &= -12.
\end{array}$

:::{dropdown} Solution
Here $A = \begin{pmatrix} -2 & -3 & -1 \\ -4 & 4 & 3 \\ -3 & 0 & 0 \end{pmatrix}$ and $\mathbf{b} = \begin{pmatrix} -5 \\ -20 \\ -12 \end{pmatrix}$

$$ \begin{align*}
    x_1 &= \frac{
    \begin{vmatrix}-5 & -3 & -1 \\ -20 & 4 & 3 \\ -12 & 0 & 0 \end{vmatrix}}
    {\begin{vmatrix} -2 & -3 & -1 \\ -4 & 4 & 3 \\ -3 & 0 & 0 \end{vmatrix}}
    = \frac{-12
    \begin{vmatrix} -3 & -1 \\ 4 & 3 \end{vmatrix}}
    {-3\begin{vmatrix} -3 & -1 \\ 4 & 3 \end{vmatrix}} \\
    &= \frac{-12(-5)}{-3(-5)} = \frac{60}{15} = 4,\\ \\
    x_2 &= \frac{
    \begin{vmatrix} -2 & -5 & -1 \\ -4 & -20 & 3 \\ -3 & -12 & 0 \end{vmatrix}}{15} 
    = \frac{-\begin{vmatrix} -4 & -20 \\ -3 & -12 \end{vmatrix} 
    - 3\begin{vmatrix}-2 & -5 \\ -3 & -12 \end{vmatrix}}{15}  \\
    &= \frac{12 - 3(9)}{15} = \frac{-15}{15} = -1, \\ \\
    x_3 &= \frac{
    \begin{vmatrix} -2 & -3 & - 5 \\ -4 & 4 & -20 \\ -3 & 0 & -12 \end{vmatrix}}{15}
    =\frac{-3\begin{vmatrix} -3 & -5 \\ 4 & -20 \end{vmatrix} - 
    12\begin{vmatrix} -2 & -3 \\ -4 & 4 \end{vmatrix}}{15} \\
    & = \frac{-3(80) - 12(-20)}{15} = \frac{0}{15} = 0.
\end{align*} $$

Checking the solution

$$ \begin{align*}
    A\mathbf{x} = 
    \begin{pmatrix} -2 & -3 & -1 \\ -4 & 4 & 3 \\ -3 & 0 & 0 \end{pmatrix}
    \begin{pmatrix} 4 \\ -1 \\ 0 \end{pmatrix} =
    \begin{pmatrix} -5 \\ -20 \\ -12 \end{pmatrix} = \mathbf{b} \qquad \checkmark
\end{align*} $$
:::
::::
